Veritas.Verifier.Global.fst
@@ -1,17 +1,57 @@
 module Veritas.Verifier.Global
 
+let lemma_prefix_verifiable (gl: verifiable_log) (i:seq_index gl{i > 0}):
+  Lemma (verifiable (prefix gl i)) = 
+  let pgl = prefix gl i in
+  let aux (tid:seq_index pgl):
+    Lemma (requires True)
+          (ensures (VT.verifiable (thread_log pgl tid)))
+          [SMTPat (VT.verifiable (thread_log pgl tid))] = 
+    assert(thread_log pgl tid = thread_log gl tid);
+    ()
+  in
+  ()
+
+let rec hadd_aux (gl: verifiable_log): 
+  Tot (ms_hash_value)
+  (decreases (length gl)) = 
+  let p = length gl in
+  if p = 1 then 
+    thread_hadd (VT.verify (thread_log gl 0))  
+  else  (
+    let gl': g_vlog = prefix gl (p - 1) in
+    lemma_prefix_verifiable gl (p - 1);
+    let h1 = hadd_aux gl' in
+    let h2 = thread_hadd (VT.verify (thread_log gl (p - 1))) in
+    ms_hashfn_agg h1 h2
+  )
+
 (* aggregate hadd over all verifier threads *)
 let hadd (gl: verifiable_log): ms_hash_value =
-  let th = fun (tl:VT.verifiable_log) -> (thread_hadd (t_verify (fst tl) (snd tl))) in
-  let f = fun (tl:VT.verifiable_log) (h:ms_hash_value) -> (ms_hashfn_agg (th tl) h) in
-  reduce empty_hash_value f (verifiable_threads gl)
+  hadd_aux gl
+
+let rec hevict_aux (gl: verifiable_log): 
+  Tot (ms_hash_value)
+  (decreases (length gl)) = 
+  let p = length gl in
+  if p = 1 then 
+    thread_hevict (VT.verify (thread_log gl 0))  
+  else  (
+    let gl': g_vlog = prefix gl (p - 1) in
+    lemma_prefix_verifiable gl (p - 1);
+    let h1 = hevict_aux gl' in
+    let h2 = thread_hevict (VT.verify (thread_log gl (p - 1))) in
+    ms_hashfn_agg h1 h2
+  )
 
 (* aggregate hadd over all verifier threads *)
 let hevict (gl: verifiable_log): ms_hash_value =
-  let th = fun (tl:VT.verifiable_log) -> (thread_hevict (t_verify (fst tl) (snd tl))) in
-  let f = fun (tl:VT.verifiable_log) (h:ms_hash_value) -> (ms_hashfn_agg (th tl) h) in
-  reduce empty_hash_value f (verifiable_threads gl)
+  hevict_aux gl
 
-let clock (gl: verifiable_log) (i: sseq_index gl): timestamp = admit()
+let clock (gl: verifiable_log) (i: sseq_index gl): timestamp = 
+  let (tid, idx) = i in  
+  let tl = thread_log gl tid in
+  VT.clock tl idx
 
 let time_seq_ctor (gl: verifiable_log): (interleave_ctor gl) = admit()
+
