Veritas.Verifier.TSLog.fsti
@@ -21,12 +21,22 @@ module S = FStar.Seq
 module VT = Veritas.Verifier.Thread
 module VG = Veritas.Verifier.Global
 
+(* valid thread id given a number of threads *)
+let valid_tid (p:pos) = tid:nat{tid < p}
+
+(* vlog entry and tid that it went to *)
+let vlog_entry_tid (p:pos) = idx_elem #vlog_entry p
+
+(* cast to vlog entry *)
+let to_vlog_entry (#p:pos) (e: vlog_entry_tid p): vlog_entry = 
+  fst e
+
 (* 
  * an indexed sequence log represents and interleaving of a global log (a sequence of thread-level
  * verifier logs. It is a sequence of the form (e,tid) where e denotes a verifier log entry
  * and tid denotes the verifier thread that the entry comes from
  *)
-let idx_seq_vlog (p:pos) = seq (idx_elem #vlog_entry p)
+let idx_seq_vlog (p:pos) = seq (vlog_entry_tid p)
 
 (* 
  * an idx_seq_vlog is verifiable if the global sequence of logs that results from partitioning 
@@ -52,31 +62,134 @@ val lemma_prefix_verifiable (#p:pos) (itsl: its_log p) (i:nat{i <= length itsl})
         (ensures (verifiable (prefix itsl i)))
         [SMTPat (prefix itsl i)]
 
-(* extended time sequence log (with evict values) *)
-val time_seq_ext (#p:pos) (itsl: its_log p):
-  Tot (le:vlog_ext{project_seq itsl = to_vlog le})
+(* create a ts log *)
+val create (gl: VG.verifiable_log): its_log (length gl)
 
-val lemma_its_prefix_ext (#n:pos) (itsl:its_log n) (i:nat{i <= length itsl}):
-  Lemma (requires True)
-        (ensures (time_seq_ext (prefix itsl i) = prefix (time_seq_ext itsl) i))
-        [SMTPat (time_seq_ext (prefix itsl i))]
+(* get back the verifier logs from ts log *)
+let to_g_vlog (#p:pos) (itsl: its_log p): VG.verifiable_log =
+  partition_idx_seq itsl
 
-let is_eac_log (#p:pos) (itsl: its_log p):bool = E.is_eac_log (time_seq_ext itsl)
+(* we get back the global logs used to crate ts log with t_g_vlog *)
+val lemma_create_correct (gl: VG.verifiable_log):
+  Lemma (gl = to_g_vlog (create gl))
 
-type eac_ts_log (p:pos) = itsl: its_log p {is_eac_log itsl}
-type non_eac_ts_log (p:pos) = itsl: its_log p {not (is_eac_log itsl)}
+(* the log entry referenced by the ith entry *)
+let vlog_entry_at (#p:pos) (itsl: its_log p) (i: seq_index itsl): vlog_entry =
+  fst (index itsl i)
+
+(* the key referenced by the i'th entry *)
+let key_of (#p:pos) (e: vlog_entry_tid p): key =
+  V.key_of (to_vlog_entry e)
+
+let key_at (#p:pos) (itsl: its_log p) (i: seq_index itsl): key = 
+  V.key_of (vlog_entry_at itsl i)
+
+let is_add (#p:pos) (e: vlog_entry_tid p): bool = 
+  V.is_add (fst e)
+
+let is_add_of_key (#p:pos) (k:key) (e: vlog_entry_tid p): bool = 
+  is_add e && 
+  key_of e = k
+
+(* is the i'th index of itsl a blum add *)
+let is_blum_add (#p:pos) (ie:vlog_entry_tid p):bool =
+  let (e,_) = ie in
+  match e with
+  | AddB _ _ _ -> true
+  | _ -> false
+
+let is_evict (#p:pos) (e:vlog_entry_tid p): bool = 
+  V.is_evict (to_vlog_entry e)
+
+(* is the index i of ts log an blum evict *)
+let is_blum_evict (#p:pos) (ie:vlog_entry_tid p): bool = 
+  let (e,_) = ie in
+  match e with
+  | EvictB _ _ -> true
+  | EvictBM _ _ _ -> true
+  | _ -> false
+
+let is_evict_of_key (k:key) (#p:pos) (ie:vlog_entry_tid p): bool = 
+  is_evict ie &&
+  key_of ie = k
+  
+let has_next_add_of_key (#p:pos) (itsl: its_log p) (i:seq_index itsl) (k:key): bool =
+  has_next (is_add_of_key k) itsl i
+
+let next_add_of_key (#p:pos) 
+  (itsl: its_log p) 
+  (i:seq_index itsl) (k:key{has_next_add_of_key itsl i k}): 
+  (j:seq_index itsl{j > i && is_add_of_key k (index itsl j)}) = 
+  next_index (is_add_of_key k) itsl i
+
+let is_entry_of_key (k:key) (#p:pos) (e:vlog_entry_tid p): bool = 
+  key_of e = k
+
+let has_some_entry_of_key (#p:pos) (itsl: its_log p) (k:key): bool = 
+  exists_sat_elems (is_entry_of_key k) itsl
+
+let last_idx_of_key (#p:pos) (itsl: its_log p) (k:key{has_some_entry_of_key itsl k}):
+  seq_index itsl = 
+  last_index (is_entry_of_key k) itsl
+
+let add_method_of (#p:pos) (e:vlog_entry_tid p{is_add e}): add_method = 
+  V.addm_of_entry (to_vlog_entry e)
+
+(* does the key k have some add *)
+let has_some_add_of_key (#p:pos) (itsl: its_log p) (k:key): bool = 
+  exists_sat_elems (is_add_of_key k) itsl
+
+(* when the eac state of a key is instore return the index of the last add that transitioned
+ * the key k to "instore" *)
+val last_add_idx (#p:pos) (itsl: its_log p) (k: key{has_some_add_of_key itsl k}): 
+  (i:seq_index itsl{is_add_of_key k (index itsl i)})
+
+(* thread id of the ith entry *)
+let thread_id_of (#p:pos) (itsl: its_log p) (i: seq_index itsl): valid_tid p =
+  snd (index itsl i)  
+
+(* the verifier thread where the last add of key k happens *)
+let last_add_tid (#p:pos) (itsl: its_log p) (k: key{has_some_add_of_key itsl k}): valid_tid p =
+  thread_id_of itsl (last_add_idx itsl k)
+
+(*thread state after processing ts log - guaranteed to be valid *)
+val thread_state (#p:pos) (itsl: its_log p) (tid: valid_tid p): (vs:vtls{Valid? vs})
+
+(* thread store after processing ts log *)
+let thread_store (#p:pos) (itsl: its_log p) (tid: valid_tid p): vstore =
+  Valid?.st (thread_state itsl tid)
+
+(* 
+ * let tid = thread_id_of itsl i. 
+ * this lemma states that state of tid at (i+1) is obtained by the state at (i) 
+ * applying the vlog entry at i.
+ *)
+val lemma_verifier_thread_state_extend (#p:pos) (itsl: its_log p) (i:seq_index itsl):
+  Lemma (thread_state (prefix itsl (i + 1)) (thread_id_of itsl i)== 
+         t_verify_step (thread_state (prefix itsl i) (thread_id_of itsl i))
+                       (vlog_entry_at itsl i))
+
+(* is this an evict add consistent log *)
+val is_eac (#p:pos) (itsl: its_log p):bool
+
+(* eac ts log *)
+let eac_log (p:pos) = itsl: its_log p {is_eac itsl}
+
+(* non-eac ts log *)
+type neac_log (p:pos) = itsl: its_log p {not (is_eac itsl)}
 
 (* if itsl is eac, then any prefix is also eac *)
-val lemma_eac_implies_prefix_eac (#p:pos) (itsl: eac_ts_log p) (i:nat {i <= length itsl}):
+val lemma_eac_implies_prefix_eac (#p:pos) (itsl: eac_log p) (i:nat {i <= length itsl}):
   Lemma (requires True)
-        (ensures (is_eac_log (prefix itsl i)))
+        (ensures (is_eac (prefix itsl i)))
         [SMTPat (prefix itsl i)]
 
 (* the eac state of a key at the end of an its log *)
-let eac_state_of_key (#p:pos) (itsl: its_log p) (k:key): eac_state = 
-  let tsle = time_seq_ext itsl in 
-  let tslek = partn eac_sm k tsle in
-  seq_machine_run eac_smk tslek
+val eac_state_of_key (#p:pos) (itsl: its_log p) (k:key): eac_state 
+
+(* by definition, ts log is eac_valid only if the state of each key is not EACFail *)
+val lemma_eac_state_of_key_valid (#p:pos) (itsl: eac_log p) (k:key):
+  Lemma (EACFail <> eac_state_of_key itsl k)
 
 (* is the eac state of key at the end of its_log init *)
 let is_eac_state_init (#p:pos) (itsl: its_log p) (k:key): bool =
@@ -111,173 +224,120 @@ let is_eac_state_evicted_blum (#p:pos) (itsl: its_log p) (k:key): bool =
 let is_eac_state_instore (#p:pos) (itsl: its_log p) (k:key):bool = 
   EACInStore? (eac_state_of_key itsl k)
 
-(* the state of a verifier thread after processing entries in a log *)
-let verifier_thread_state (#p:pos) (itsl: its_log p) (id:nat{id < p}): (st:vtls{Valid? st}) = 
-  let gl = partition_idx_seq itsl in
-  assert(VT.verifiable (index (attach_index gl) id));
-  t_verify id (index gl id)
+let is_eac_state_active (#p:pos) (itsl: its_log p) (k:key): bool = 
+  is_eac_state_evicted itsl k ||
+  is_eac_state_instore itsl k
+
+(* the extended vlog entry to use for eac checking *)
+val vlog_entry_ext_at (#p:pos) (itsl: its_log p) (i:seq_index itsl): 
+  (e:vlog_entry_ext{E.to_vlog_entry e = vlog_entry_at itsl i})
+
+(* the eac state transition induced by the i'th entry *)
+val lemma_eac_state_transition (#p:pos) (itsl: its_log p) (i:seq_index itsl):
+  Lemma (eac_state_of_key (prefix itsl (i + 1)) (key_at itsl i) = 
+         eac_add (vlog_entry_ext_at itsl i) 
+                 (eac_state_of_key (prefix itsl i) (key_at itsl i)))
+
+(* when the eac state of a key is "instore" then there is always a previous add *)
+val lemma_eac_state_active_implies_prev_add (#p:pos) (itsl: eac_log p) 
+  (k:key{is_eac_state_active itsl k}):
+  Lemma (requires True)
+        (ensures (has_some_add_of_key itsl k))
+        [SMTPat (is_eac_state_instore itsl k)]
+
+(* add method of an eac state *)
+val lemma_eac_state_addm (#p:pos) (itsl: eac_log p) (k:key{is_eac_state_instore itsl k}):
+  Lemma (E.add_method_of (eac_state_of_key itsl k) = 
+         add_method_of (index itsl (last_add_idx itsl k)))
+
+(* the evicted value is always of the correct type for the associated key *)
+val lemma_eac_value_correct_type (#p:pos) (itsl: eac_log p) (k:key):  
+  Lemma (requires (E.is_eac_state_active (eac_state_of_key itsl k)))
+        (ensures is_value_of k (E.value_of (eac_state_of_key itsl k)))
+
+(* value associated with eac state *)
+val eac_state_value (#n:pos) (itsl: eac_log n) (k:key{is_eac_state_active itsl k}): value_type_of k
+
+(* we never see operations on Root so its eac state is always init *)
+val lemma_eac_state_of_root_init (#p:pos) (itsl: eac_log p):
+  Lemma (is_eac_state_init itsl Root)
 
 (* 
  * when the eac state of a key is Init (no operations on the key yet) no 
- * thread contains the key in its store 
+ * thread contains the key in its store. Valid only for non-root keys 
+ * since we start off with the root in the cache of thread 0
  *)
-val lemma_eac_state_init_store 
-   (#p:pos) 
-   (itsl: eac_ts_log p) (k: key{k <> Root && is_eac_state_init itsl k}) (id:nat{id < p}):
-   Lemma (not (store_contains (thread_store (verifier_thread_state itsl id)) k)) 
+val lemma_eac_state_init_store (#p:pos) (itsl: eac_log p) (k: key) (tid:valid_tid p):
+  Lemma (requires (k <> Root && is_eac_state_init itsl k))
+        (ensures (not (store_contains (thread_store itsl tid) k)))
 
-(* when the eac state of a key is EACEvicted then no thread contains the key in its store *)
-val lemma_eac_state_evicted_store (#p:pos) (itsl: eac_ts_log p) 
-  (k: key{is_eac_state_evicted itsl k}) (id:nat{id < p}):
-  Lemma (not (store_contains (thread_store (verifier_thread_state itsl id)) k))
-  
-(* when the eac state of a key is "instore" then there is always a previous add *)
-val lemma_eac_state_instore_implies_prev_add (#p:pos) (itsl: eac_ts_log p) 
-  (k:key{is_eac_state_instore itsl k}):
-  Lemma (has_some_add_of_key k (project_seq itsl))
+(* when the eac state of a key is evicted then no thread contains the key in its store *)
+val lemma_eac_state_evicted_store  (#p:pos) (itsl: eac_log p) (k: key{is_eac_state_evicted itsl k}) 
+  (tid:valid_tid p):
+  Lemma (not (store_contains (thread_store itsl tid) k))
 
-(* when the eac state of a key is instore return the index of the last add that transitioned
- * the key k to "instore" *)
-let last_add_idx (#p:pos) (itsl: eac_ts_log p) (k: key{is_eac_state_instore itsl k}): seq_index itsl =
-   lemma_eac_state_instore_implies_prev_add itsl k;
-   last_index (is_add_of_key k) (project_seq itsl)
+(* when the eac_state of k is instore, then k is in the store of a unique verifier thread *)
+val stored_tid (#p:pos) (itsl: eac_log p) (k:key{is_eac_state_instore itsl k}): 
+  (tid: valid_tid p{store_contains (thread_store itsl tid) k})
 
-(* the verifier thread where the last add of key k happens *)
-let last_add_tid (#p:pos) (itsl: eac_ts_log p) (k: key{is_eac_state_instore itsl k}): (tid:nat{tid < p}) =
-  snd (index itsl (last_add_idx itsl k))
+(* uniqueness: k is not in any store other than stored_tid *)
+val lemma_key_in_unique_store (#p:pos) (itsl: eac_log p) (k:key) (tid: valid_tid p):
+  Lemma (requires (is_eac_state_instore itsl k /\ tid <> stored_tid itsl k))
+        (ensures (not (store_contains (thread_store itsl tid) k)))
 
-(* if the eac_state of k is instore, then that k is in the store of the verifier thread of its last add *)
-val lemma_eac_state_instore (#p:pos) (itsl: eac_ts_log p) (k:key{is_eac_state_instore itsl k}):
-  Lemma (store_contains (thread_store (verifier_thread_state itsl (last_add_tid itsl k))) k /\
-         stored_value (thread_store (verifier_thread_state itsl (last_add_tid itsl k))) k = 
-         EACInStore?.v (eac_state_of_key itsl k))
+(* it is therefore meaningful to talk of the stored value of a key *)
+let stored_value (#p:pos) (itsl: eac_log p) (k:key{is_eac_state_instore itsl k}): value_type_of k =
+  V.stored_value (thread_store itsl (stored_tid itsl k)) k
 
-val lemma_eac_state_instore_addm (#p:pos) (itsl: eac_ts_log p) (k:key{is_eac_state_instore itsl k}):
-  Lemma (is_add (index (project_seq itsl) (last_add_idx itsl k)) /\
-         store_contains (thread_store (verifier_thread_state itsl (last_add_tid itsl k))) k /\
-         EACInStore?.m (eac_state_of_key itsl k) = 
-         addm_of_entry (index (project_seq itsl) (last_add_idx itsl k)) /\
-         EACInStore?.m (eac_state_of_key itsl k) = 
-         add_method_of (thread_store (verifier_thread_state itsl (last_add_tid itsl k))) k)
-  
-(* if the eac state of k is instore, then k is not in the store of any verifier thread other than 
- * its last add thread *)
-val lemma_eac_state_instore2 (#p:pos) (itsl: eac_ts_log p) 
-  (k:key{is_eac_state_instore itsl k}) (id:nat{id < p}):
-  Lemma (requires (id <> last_add_tid itsl k))
-        (ensures (not (store_contains (thread_store (verifier_thread_state itsl id)) k)))
+let stored_add_method (#p:pos) (itsl: eac_log p) (k:key {is_eac_state_instore itsl k}): add_method =
+  V.add_method_of (thread_store itsl (stored_tid itsl k)) k
 
-(* if k is in a verifier store, then its eac_state is instore *)
-val lemma_instore_implies_eac_state_instore (#p:pos) (itsl:eac_ts_log p) (k:key{k <> Root}) (tid:nat{tid < p}):
-  Lemma (store_contains (thread_store (verifier_thread_state itsl tid)) k ==> is_eac_state_instore itsl k)
-         
-(* the root is always in thread 0 *)
-val lemma_root_in_store0 (#p:pos) (itsl: eac_ts_log p):
-  Lemma (store_contains (thread_store (verifier_thread_state itsl 0)) Root)
-
-val lemma_root_not_in_store (#p:pos) (itsl: eac_ts_log p) (tid:pos {tid < p}):
-  Lemma (not (store_contains (thread_store (verifier_thread_state itsl tid)) Root))
-
-(* the evicted value is always of the correct type for the associated key *)
-val lemma_evict_value_correct_type (#p:pos) (itsl: eac_ts_log p) (k:key{is_eac_state_evicted itsl k}):
-  Lemma (is_value_of k (E.value_of (eac_state_of_key itsl k)))
+(* for data keys, the value in the store is the same as the value associated with the eac state *)
+val lemma_eac_stored_value (#p:pos) (itsl: eac_log p) (k: data_key{is_eac_state_instore itsl k}):
+  Lemma (eac_state_value itsl k = stored_value itsl k)
 
 (* 
- * for keys in a thread store, return the value in the thread store; 
- * for other keys return the last evict value or null (init)
+ * for all keys, the add method stored in the store is the same as the add method associated 
+ * with eac state
  *)
-val eac_value (#n:pos) (itsl: eac_ts_log n) (k:key): value_type_of k
+val lemma_eac_stored_addm (#p:pos) (itsl: eac_log p) (k:key{is_eac_state_instore itsl k}):
+  Lemma (E.add_method_of (eac_state_of_key itsl k) = stored_add_method itsl k)
+  
+(* if k is in a verifier store, then its eac_state is instore *)
+val lemma_instore_implies_eac_state_instore (#p:pos) (itsl:eac_log p) (k:key{k <> Root}) (tid:valid_tid p):
+  Lemma (store_contains (thread_store itsl tid) k ==> is_eac_state_instore itsl k)
+         
+(* the root is always in thread 0 *)
+val lemma_root_in_store0 (#p:pos) (itsl: eac_log p):
+  Lemma (store_contains (thread_store itsl 0) Root)
 
-val lemma_eac_value_is_stored_value (#p:pos) (itsl: eac_ts_log p) (k:key) (id:nat{id < p}):
-  Lemma (requires (store_contains (thread_store (verifier_thread_state itsl id)) k))
-        (ensures (eac_value itsl k = 
-                  stored_value (thread_store (verifier_thread_state itsl id)) k))
+val lemma_root_not_in_store (#p:pos) (itsl: eac_log p) (tid:valid_tid p):
+  Lemma (not (store_contains (thread_store itsl tid) Root))
 
-val lemma_eac_value_is_evicted_value (#p:pos) (itsl: eac_ts_log p) (k:key):
+(* we use eac constraints to associate a value with each key *)
+val eac_value (#p:pos) (itsl: eac_log p) (k:key): value_type_of k
+
+(* eac_value is consistent with stored value *)
+val lemma_eac_value_is_stored_value (#p:pos) (itsl: eac_log p) (k:key) (tid: valid_tid p):  
+  Lemma (requires (store_contains (thread_store itsl tid) k))
+        (ensures (eac_value itsl k = V.stored_value (thread_store itsl tid) k))
+
+val lemma_eac_value_is_evicted_value (#p:pos) (itsl: eac_log p) (k:key):
   Lemma (requires (is_eac_state_evicted itsl k))
-        (ensures (eac_state_evicted_value itsl k = eac_value itsl k))
-
-let key_of (#p:pos) (ie:idx_elem #vlog_entry p): key = 
-  let (e,_) = ie in
-  V.key_of e
-
-let entry_of_key (k:key) (#p:pos) (ie:idx_elem #vlog_entry p): bool = 
-  let (e,_) = ie in
-  V.key_of e = k
-
-let has_some_entry_of_key (#p:pos) (itsl: its_log p) (k:key): bool = 
-  exists_sat_elems (entry_of_key k) itsl
-
-let its_vlog_entry (#n:pos) (itsl: its_log n) (i:seq_index itsl): vlog_entry =
-  fst (index itsl i)
-
-let its_thread_id (#n:pos) (itsl: its_log n) (i:seq_index itsl): (tid:nat{tid < n}) =
-  snd (index itsl i)
+        (ensures (eac_state_evicted_value itsl k = eac_state_value itsl k))
 
 val lemma_ext_evict_val_is_stored_val (#p:pos) (itsl: its_log p) (i: seq_index itsl):
-  Lemma (requires (is_evict (fst (index itsl i))))
-        (ensures (is_evict_ext (index (time_seq_ext itsl) i) /\
-                  store_contains (thread_store (verifier_thread_state (prefix itsl i)
-                                                                      (snd (index itsl i))))
-                                 (V.key_of (fst (index itsl i))) /\
-                  value_ext (index (time_seq_ext itsl) i) = 
-                  stored_value (thread_store (verifier_thread_state (prefix itsl i)
-                                                                    (snd (index itsl i))))
-                               (V.key_of (fst (index itsl i)))))
-
-let is_of_key (k:key) (#p:pos) (ie:idx_elem #vlog_entry p): bool = 
-  let (e,_) = ie in
-  V.is_of_key e k
-
-let is_add (#p:pos) (ie:idx_elem #vlog_entry p): bool = 
-  let (e,_) = ie in
-  V.is_add e
-
-let is_evict (#p:pos) (ie:idx_elem #vlog_entry p): bool = 
-  let (e,_) = ie in
-  V.is_evict e
-
-(* is the i'th index of itsl a blum add *)
-let is_blum_add (#p:nat) (ie:idx_elem #vlog_entry p):bool =
-  let (e,_) = ie in
-  match e with
-  | AddB _ _ _ -> true
-  | _ -> false
-
-(* is the index i of ts log an blum evict *)
-let is_blum_evict (#p:pos) (ie:idx_elem #vlog_entry p): bool = 
-  let (e,_) = ie in
-  match e with
-  | EvictB _ _ -> true
-  | EvictBM _ _ _ -> true
-  | _ -> false
-
-let is_add_of_key (k:key) (#p:pos) (ie:idx_elem #vlog_entry p): bool = 
-  is_add ie &&
-  is_of_key k ie
-
-let is_evict_of_key (k:key) (#p:pos) (ie:idx_elem #vlog_entry p): bool = 
-  is_evict ie &&
-  is_of_key k ie
-  
-let has_next_add_of_key (#p:pos) (itsl: its_log p) (i:seq_index itsl) (k:key): bool =
-  has_next (is_add_of_key k) itsl i
-
-let next_add_of_key (#p:pos) 
-  (itsl: its_log p) 
-  (i:seq_index itsl) (k:key{has_next_add_of_key itsl i k}): 
-  (j:seq_index itsl{j > i && is_add_of_key k (index itsl j)}) = 
-  next_index (is_add_of_key k) itsl i
-
-let last_idx_of_key (#p:pos) (itsl: its_log p) (k:key{has_some_entry_of_key itsl k}):
-  seq_index itsl = 
-  last_index (entry_of_key k) itsl
+  Lemma (requires (is_evict (index itsl i)))
+        (ensures (store_contains (thread_store itsl (thread_id_of itsl i)) (key_at itsl i) /\
+                  is_evict_ext (vlog_entry_ext_at itsl i) /\
+                  V.stored_value (thread_store itsl (thread_id_of itsl i)) (key_at itsl i) = 
+                  value_ext (vlog_entry_ext_at itsl i)))
 
 (* if an evict is not the last entry of a key, then there is a add subsequent to the 
  * evict *)
 val lemma_evict_has_next_add (#p:pos) (itsl: its_log p) (i:seq_index itsl):
   Lemma (requires (is_evict (index itsl i) /\
-                   exists_sat_elems (entry_of_key (key_of (index itsl i))) itsl) /\
+                   exists_sat_elems (is_entry_of_key (key_of (index itsl i))) itsl) /\
                    i < last_idx_of_key itsl (key_of (index itsl i)))
         (ensures (has_next_add_of_key itsl i (key_of (index itsl i))))
 
